# Common Formulas

$$a^2 - b^2 = (a+b)(a-b)$$
$$a^2 \pm 2ab + b^2 = (a\pm b)^2$$
$$a^3\pm 3a^2b + 3ab^2 \pm b^3 = (a\pm b)^2$$
$$a^3 + b^3 = (a + b)(a^2 - ab + b^2)$$
$$a^3 - b^3 = (a-b)(a^2 + ab + b^2)$$
$$(a+b+c)^2 = a^2 + b^2 + c^2 + 2ab + 2bc + 2ca$$
$$a^3 + b^3 + c^3 - 3abc = (a+b+c)(a^2 + b^2 + c^2 - ab - bc - ca)$$
$$a^n - b^n = (a-b)(a^{n-1} + a^{n-2}b + a^{n-3}{b^2} + ... + ab^{n-2} + b^{n-1})$$
$$a^n - b^n = (a+b)(a^{n-1} - a^{n-2}b + a^{n-3}{b^2} - ... + ab^{n-2} - b^{n-1})\; n \in \mathbb{N} \;\text{even}$$
$$a^n + b^n = (a+b)(a^{n-1} - a^{n-2}b + a^{n-3}{b^2} - ... - ab^{n-2} + b^{n-1})\; n \in \mathbb{N} \;\text{odd}$$
